silveroak-opentitan/aes/Acorn/CipherEquivalence.v
@@ -1,0 +1,79 @@
+(****************************************************************************)
+(* Copyright 2020 The Project Oak Authors                                   *)
+(*                                                                          *)
+(* Licensed under the Apache License, Version 2.0 (the "License")           *)
+(* you may not use this file except in compliance with the License.         *)
+(* You may obtain a copy of the License at                                  *)
+(*                                                                          *)
+(*     http://www.apache.org/licenses/LICENSE-2.0                           *)
+(*                                                                          *)
+(* Unless required by applicable law or agreed to in writing, software      *)
+(* distributed under the License is distributed on an "AS IS" BASIS,        *)
+(* WITHOUT WARRANTIES OR CONDITIONS OF ANY KIND, either express or implied. *)
+(* See the License for the specific language governing permissions and      *)
+(* limitations under the License.                                           *)
+(****************************************************************************)
+
+Require Import Coq.Lists.List.
+Require Import Coq.Vectors.Vector.
+Require Import ExtLib.Structures.Monads.
+Require Import Cava.ListUtils.
+Require Import Cava.VectorUtils.
+Require Import Cava.Monad.MonadFacts.
+Require Import Cava.Acorn.Acorn.
+Require Import Cava.Acorn.Lib.AcornVectors.
+Require Import Cava.Acorn.Combinational.
+
+Require Import AesSpec.Cipher.
+Require Import AcornAes.CipherRound.
+
+Import MonadNotation.
+Existing Instance Combinational.
+
+Section WithSubroutines.
+  Local Notation byte := (t bool 8).
+  Local Notation state := (t (t byte 4) 4) (only parsing).
+  Local Notation key := (t (t byte 4) 4) (only parsing).
+  Context (sub_bytes:     state -> ident state)
+          (shift_rows:    state -> ident state)
+          (mix_columns:   state -> ident state).
+  Let add_round_key : key -> state -> ident state := xor4x4V.
+
+  Let sub_bytes' : state -> state := (fun st => unIdent (sub_bytes st)).
+  Let shift_rows' : state -> state := (fun st => unIdent (shift_rows st)).
+  Let mix_columns' : state -> state := (fun st => unIdent (mix_columns st)).
+  (* Note: argument order is switched for spec *)
+  Let add_round_key' : state -> key -> state :=
+    (fun st k => unIdent (add_round_key k st)).
+
+  Lemma cipher_equiv
+        (first_key last_key : key) (middle_keys : list key) (input : state) :
+    let cipher := (cipher sub_bytes shift_rows mix_columns add_round_key) in
+    let cipher_spec := (Cipher.cipher _ _ add_round_key'
+                                      sub_bytes' shift_rows' mix_columns') in
+    unIdent (cipher first_key last_key middle_keys input)
+    = cipher_spec first_key last_key middle_keys input.
+  Proof.
+    cbv zeta. subst sub_bytes' shift_rows' mix_columns' add_round_key' add_round_key.
+    cbv [cipher cipher_round Cipher.cipher]. cbn [bind ret Monad_ident unIdent].
+    repeat (f_equal; [ ]). rewrite foldLM_ident_fold_left.
+    eapply fold_left_preserves_relation; [ reflexivity | ].
+    intros; subst. reflexivity.
+  Qed.
+
+  Lemma cipher_alt_equiv
+        (first_key last_key : key) (middle_keys : list key) (input : state) :
+    let cipher := (cipher_alt sub_bytes shift_rows mix_columns add_round_key) in
+    let cipher_spec := (Cipher.cipher _ _ add_round_key'
+                                      sub_bytes' shift_rows' mix_columns') in
+    unIdent (cipher first_key last_key middle_keys input)
+    = cipher_spec first_key last_key middle_keys input.
+  Proof.
+    cbv zeta. subst sub_bytes' shift_rows' mix_columns' add_round_key' add_round_key.
+    cbv [cipher_alt cipher_round Cipher.cipher].
+    cbn [bind ret Monad_ident unIdent mcompose].
+    repeat (f_equal; [ ]). rewrite foldLM_ident_fold_left.
+    eapply fold_left_preserves_relation; [ reflexivity | ].
+    intros; subst. reflexivity.
+  Qed.
+End WithSubroutines.
